theories/STLC.v
@@ -1,0 +1,101 @@
+
+Require Import List.
+Import ListNotations.
+Require Import String.
+From MasterThesis Require Import
+     Context.
+Import ctx.notations.
+
+(* =================================== *)
+(*  The Simply-Typed Lambda Calculus   *)
+(*      extended with Booleans         *)
+(* =================================== *)
+
+
+(* ===== Language ===== *)
+
+  Inductive ty : Type :=
+    | ty_bool : ty
+    | ty_func : ty -> ty -> ty.
+
+  Inductive expr : Type :=
+    (* values *)
+    | v_true  : expr
+    | v_false : expr
+    (* compound expressions *)
+    | e_if    : expr -> expr -> expr -> expr
+    | e_var   : string -> expr
+    | e_absu  : string -> expr -> expr
+    | e_abst  : string -> ty -> expr -> expr
+    | e_app   : expr -> expr -> expr.
+
+(* ===== Typing relation ===== *)
+
+  (* Context/environment of term variables and their types *)
+  Definition env := list (string * ty).
+
+  Fixpoint value {X: Type} (var : string) (ctx : list (string * X)) : option X :=
+    match ctx with
+    | nil => None
+    | (var', val) :: ctx' =>
+        if (string_dec var var') then Some val else (value var ctx')
+    end.
+
+  Reserved Notation "G |-- E ; T ~> EE"
+              (at level 50).
+
+  Inductive tpb : env -> expr -> ty -> expr -> Prop :=
+    | tpb_false : forall g,
+        g |-- v_false ; ty_bool ~> v_false
+    | tpb_true : forall g,
+        g |-- v_true ; ty_bool ~> v_true
+    | tpb_if : forall g cnd cnd' coq coq' alt alt' t,
+        g |-- cnd ; ty_bool ~> cnd' ->
+        g |-- coq ; t       ~> coq' ->
+        g |-- alt ; t       ~> alt' ->
+        g |-- (e_if cnd coq alt) ; t ~> (e_if cnd' coq' alt')
+    | tpb_var : forall g v vt,
+        value v g = Some vt ->
+        g |-- (e_var v) ; vt ~> (e_var v)
+    | tpb_absu : forall v vt g e e' t,
+        ((v, vt) :: g) |-- e ; t ~> e' ->
+        g |-- (e_absu v e) ; (ty_func vt t) ~> (e_abst v vt e')
+    | tpb_abst : forall v vt g e e' t,
+        ((v, vt) :: g) |-- e ; t ~> e' ->
+        g |-- (e_abst v vt e) ; (ty_func vt t) ~> (e_abst v vt e')
+    | tpb_app : forall g e1 t1 e1' e2 t2 e2',
+        g |-- e1 ; (ty_func t2 t1) ~> e1' ->
+        g |-- e2 ; t2 ~> e2' ->
+        g |-- (e_app e1 e2) ; t1 ~> (e_app e1' e2')
+
+    where "G |-- E ; T ~> EE" := (tpb G E T EE).
+
+  (* (λx : Bool . x) : Bool → Bool  ... is well-typed *)
+  Example typed_bool_id_func :
+    nil |-- (e_abst "x" ty_bool (e_var "x")) ; (ty_func ty_bool ty_bool) ~> (e_abst "x" ty_bool (e_var "x")).
+  Proof.
+    apply tpb_abst. apply tpb_var. cbn. reflexivity.
+  Qed.
+
+  (* (λx . x) : Bool → Bool  ... is well-typed *)
+  Example untyped_bool_id_func :
+    nil |-- (e_absu "x" (e_var "x")) ; (ty_func ty_bool ty_bool) ~> (e_abst "x" ty_bool (e_var "x")).
+  Proof.
+    apply tpb_absu. apply tpb_var. cbn. reflexivity.
+  Qed.
+
+Section Symbolic.
+
+  Inductive Ty (Σ : Ctx nat) : Type :=
+    | Ty_bool : Ty Σ
+    | Ty_func : Ty Σ -> Ty Σ -> Ty Σ
+    | Ty_hole : forall (i : nat), i ∈ Σ -> Ty Σ.
+
+  Definition Env Σ := list (string * Ty Σ).
+
+  Inductive Cstr (A : Ctx nat -> Type) (Σ : Ctx nat) : Type :=
+    | C_eqc : Ty Σ -> Ty Σ -> Cstr A Σ -> Cstr A Σ
+    | C_val : A Σ -> Cstr A Σ
+    | C_fls : Cstr A Σ
+    | C_exi : forall (i : nat), Cstr A (Σ ▻ i) -> Cstr A Σ.
+End Symbolic.
